Question 1: 
Expression: a + b 
Initial values: a = 3, b = 4
Math: 3 + 4 
Final result: 7


Question 2: 
Expression: -a + b
Initial values: a = 3, b = 4
Math: -3 + 4 
Final result: 1 


Question 3:
Expression: ++a + c
Initial values: a = 3, c = -2 
Step 1: ++a → prefix increment → a becomes 4 and 4 is used
Step 2: plus sign multiplied by negative two is -2
Math: 4 -2 = 2
Final Result: 2


Question 4: 
Expression: a / b 
Initial values: a = 3, b = 4
Math: 3 / 4 = 0.75
Final result: 0 


Question 5: 
Expression: b / a
Initial values: a = 3, b = 4
Math: 4 / 3 = 1.333
Final Result: 1


Question 6:
Expression: ++a + b++
Initial values: a = 3, b = 4
Step 1: ++a → prefix increment → a becomes 4 and 4 is used
Step 2: b++ → postfix increment → b stays 4 during the expression and becomes 5 afterward
Math: 4 + 4 = 8
Final result: 8
